Garden/OpenVM/BranchEq/core_expr.v
@@ -158,29 +158,6 @@ Definition eval {NUM_LIMBS : Z}
     |};
   |}.
 
-Definition print_branch_eq {NUM_LIMBS : Z} : string :=
-  let air := {|
-    BranchEqualCoreAir.offset := 12;
-    BranchEqualCoreAir.pc_step := 23;
-  |} in
-  let local : BranchEqualCoreCols.t NUM_LIMBS Var.t := {|
-    BranchEqualCoreCols.a := {| Array.get := fun i => Var.make (i + 0) |};
-    BranchEqualCoreCols.b := {| Array.get := fun i => Var.make (i + NUM_LIMBS) |};
-    BranchEqualCoreCols.cmp_result := Var.make (2 * NUM_LIMBS);
-    BranchEqualCoreCols.imm := Var.make (2 * NUM_LIMBS + 1);
-    BranchEqualCoreCols.opcode_beq_flag := Var.make (2 * NUM_LIMBS + 2);
-    BranchEqualCoreCols.opcode_bne_flag := Var.make (2 * NUM_LIMBS + 3);
-    BranchEqualCoreCols.diff_inv_marker := {| Array.get := fun i => Var.make (i + 2 * NUM_LIMBS + 4) |};
-  |} in
-  let from_pc : Var.t := Var.make (3 * NUM_LIMBS + 4) in
-  PrettyPrint.cats [
-    PrettyPrint.endl;
-    PrettyPrint.to_string (eval air local from_pc) 0;
-    PrettyPrint.endl
-  ].
-
-Compute print_branch_eq (NUM_LIMBS := 4).
-
 (** We prove the equality of the [eval] definition above with the [eval] definition directly using
     field elements. *)
 Lemma eval_eq {p} `{Prime p} {NUM_LIMBS : Z}
