Garden/OpenVM/Sha256/air_expr.v
@@ -804,37 +804,3 @@ Definition eval
       round_local_cols round_next_cols
       digest_local_cols digest_next_cols in
   MExpr.pure tt.
-
-Definition print_eval : string :=
-  let self : Sha256Air.t := {|
-    Sha256Air.bitwise_lookup_bus := {|
-      BitwiseOperationLookupBus.inner := {|
-        LookupBus.index := 8000;
-      |};
-    |};
-    Sha256Air.row_idx_encoder := row_idx_encoder;
-    Sha256Air.bus := 8001;
-  |} in
-  let start_col := 0 in
-  let '(round_local_cols, round_next_cols) :=
-    MGenerate.eval [[ (
-      MGenerate.generate (A := Sha256RoundCols.t Var.t) (||),
-      MGenerate.generate (A := Sha256RoundCols.t Var.t) (||)
-    ) ]] in
-  (* Because the "round" version is longer than the "digest" one *)
-  let digest_local_cols :=
-    MGenerate.eval [[
-      MGenerate.generate (A := Sha256DigestCols.t Var.t) (||)
-    ]] in
-  let '(_, digest_next_cols) :=
-    MGenerate.eval [[ (
-      MGenerate.generate (A := Sha256RoundCols.t Var.t) (||),
-      MGenerate.generate (A := Sha256DigestCols.t Var.t) (||)
-    ) ]] in
-  PrettyPrint.cats [
-    PrettyPrint.endl;
-    PrettyPrint.to_string (eval self start_col round_local_cols round_next_cols digest_local_cols digest_next_cols) 0;
-    PrettyPrint.endl
-  ].
-
-Compute print_eval.
