Garden/OpenVM/Sha256/pretty_print.v
@@ -1,0 +1,39 @@
+Require Import Garden.Plonky3.M.
+Require Import Garden.Plonky3.MExpr.
+Require Import Garden.OpenVM.primitives.bitwise_op_lookup.
+Require Import Garden.OpenVM.Sha256.air_expr.
+Require Import Garden.OpenVM.Sha256.columns.
+
+Definition print_eval : string :=
+  let self : Sha256Air.t := {|
+    Sha256Air.bitwise_lookup_bus := {|
+      BitwiseOperationLookupBus.inner := {|
+        LookupBus.index := 8000;
+      |};
+    |};
+    Sha256Air.row_idx_encoder := row_idx_encoder;
+    Sha256Air.bus := 8001;
+  |} in
+  let start_col := 0 in
+  let '(round_local_cols, round_next_cols) :=
+    MGenerate.eval [[ (
+      MGenerate.generate (A := Sha256RoundCols.t Var.t) (||),
+      MGenerate.generate (A := Sha256RoundCols.t Var.t) (||)
+    ) ]] in
+  (* Because the "round" version is longer than the "digest" one *)
+  let digest_local_cols :=
+    MGenerate.eval [[
+      MGenerate.generate (A := Sha256DigestCols.t Var.t) (||)
+    ]] in
+  let '(_, digest_next_cols) :=
+    MGenerate.eval [[ (
+      MGenerate.generate (A := Sha256RoundCols.t Var.t) (||),
+      MGenerate.generate (A := Sha256DigestCols.t Var.t) (||)
+    ) ]] in
+  PrettyPrint.cats [
+    PrettyPrint.endl;
+    PrettyPrint.to_string (eval self start_col round_local_cols round_next_cols digest_local_cols digest_next_cols) 0;
+    PrettyPrint.endl
+  ].
+
+Compute print_eval.
